HW2 Q1-Q2

ex2/lists.v
@@ -1,21 +1,169 @@
 Set Implicit Arguments.
 Require Import Lists.List.
+Require Import Arith.
 Import ListNotations.
-
 Print list.
 Print rev.
 
-
 (* Q1. Define `is_sorted`.  (should return a Prop.)  *)
 
+(* We define is_sorted recursively by always deconstructing one element at a time:
+   - An empty list is sorted
+   - A single element list is sorted
+   - For a non-empty list, check if head relates properly to all elements in tail *)
+Fixpoint is_sorted {A : Type} (l : list A) (R : A -> A -> Prop) : Prop :=
+  match l with
+  | [] => True
+  | x :: xs =>
+      match xs with
+      | [] => True
+      | y :: _ => R x y /\ is_sorted xs R
+      end
+  end.
 
 (* Show that this list is sorted. *)
 Lemma warm_up : is_sorted [3;5;9] le.
+Proof.
+  (* Unfold the definition *)
+  simpl.
+  split.
+  - (* 3 <= 5 *)
+    apply le_S. apply le_S. apply le_n.
+  - split.
+    + (* 5 <= 9 *)
+      apply le_S. apply le_S. apply le_S. apply le_S. apply le_n.
+    + (* is_sorted [9] le, which is True *)
+      exact I.
+Qed.
 
-
-(* Q2. Prove that an ascending list of nat, when reversed, 
+(* Q2. Prove that an ascending list of nat, when reversed,
  *     becomes a descending list. *)
 
-(*     Don't forget to use the _hint_ when proving it. *)
+(* First, let's prove that In y (rev l) <-> In y l *)
+Lemma in_rev_iff : forall {A : Type} (y : A) (l : list A),
+  In y (rev l) <-> In y l.
+Proof.
+  intros A y l.
+  induction l as [|h t IH].
+  - (* Base case: empty list *)
+    simpl. split; intro H; exact H.
+  - (* Inductive case *)
+    simpl. split.
+    + (* -> direction *)
+      intro H_in_rev.
+      rewrite in_app_iff in H_in_rev.
+      destruct H_in_rev as [H_in_rev_t | H_in_h].
+      * right. rewrite <- IH. exact H_in_rev_t.
+      * simpl in H_in_h. destruct H_in_h as [H_eq | H_false].
+        -- left. exact H_eq.
+        -- contradiction.
+    + (* <- direction *)
+      intro H_in_orig.
+      rewrite in_app_iff.
+      destruct H_in_orig as [H_eq | H_in_t].
+      * right. simpl. left. exact H_eq.
+      * left. rewrite IH. exact H_in_t.
+Qed.
 
-Theorem rev_asc_desc : ...
+(* Helper lemma: if a list is sorted ascending, then the head is <= all elements *)
+Lemma sorted_head_le_all : forall l : list nat, forall h : nat,
+  is_sorted (h :: l) le -> forall y, In y l -> h <= y.
+Proof.
+  induction l as [|h' t IH]; intros h H_sorted y H_in.
+  - (* Base case: empty tail *)
+    simpl in H_in. contradiction.
+  - (* Inductive case *)
+    simpl in H_sorted. destruct H_sorted as [H_le H_tail_sorted].
+    simpl in H_in. destruct H_in as [H_eq | H_in_t].
+    + (* y = h' *)
+      subst y. exact H_le.
+    + (* y ∈ t *)
+      (* We need to show h <= y where y ∈ t *)
+      (* We know h <= h' and the tail starting from h' is sorted *)
+      (* So we need to use transitivity: h <= h' <= y *)
+
+      (* First, let's get h' <= y from the sorted tail *)
+      assert (H_h'_le_y: h' <= y).
+      {
+        destruct t as [|h'' t'].
+        - simpl in H_in_t. contradiction.
+        - apply IH with (h := h').
+          + exact H_tail_sorted.
+          + exact H_in_t.
+      }
+
+      (* Now use transitivity *)
+      apply le_trans with h'.
+      * exact H_le.
+      * exact H_h'_le_y.
+Qed.
+
+(* Helper lemma: a sorted list appended with an element smaller than all elements
+   in the list results in a sorted list (in reverse order) *)
+Lemma sorted_app_smaller : forall l : list nat, forall x : nat,
+  is_sorted l ge ->
+  (forall y, In y l -> x <= y) ->
+  is_sorted (l ++ [x]) ge.
+Proof.
+  induction l as [|h t IH]; intros x H_sorted H_smaller.
+  - (* Base case: empty list *)
+    simpl. exact I.
+  - (* Inductive case *)
+    destruct t as [|h' t'].
+    + (* Single element case: [h] ++ [x] = [h; x] *)
+      simpl. split.
+      * (* Need to show h >= x *)
+        apply H_smaller. simpl. left. reflexivity.
+      * exact I.
+    + (* Multiple elements case *)
+      simpl. split.
+      * (* First two elements of h :: t' ++ [x] satisfy ge *)
+        simpl in H_sorted. destruct H_sorted as [H_ge H_tail_sorted].
+        exact H_ge.
+      * (* Tail is sorted *)
+        apply IH.
+        -- simpl in H_sorted. destruct H_sorted as [_ H_tail_sorted].
+           exact H_tail_sorted.
+        -- intros y H_in. apply H_smaller. simpl. right. exact H_in.
+Qed.
+
+(* Main theorem *)
+Theorem rev_asc_desc : forall l : list nat,
+  is_sorted l le -> is_sorted (rev l) ge.
+Proof.
+  induction l as [|h t IH]; intro H.
+  - (* Base case: empty list *)
+    simpl. exact I.
+  - (* Inductive case *)
+    simpl. (* rev (h :: t) = rev t ++ [h] *)
+
+    destruct t as [|h' t'].
+    + (* Single element case *)
+      simpl. exact I.
+    + (* Multiple elements case *)
+      (* We have: is_sorted (h :: h' :: t') le *)
+      (* Need to show: is_sorted (rev (h' :: t') ++ [h]) ge *)
+
+      (* Apply inductive hypothesis to get sorted tail *)
+      assert (H_rev_sorted: is_sorted (rev (h' :: t')) ge).
+      {
+        apply IH.
+        simpl in H. destruct H as [H_le H_tail_sorted].
+        exact H_tail_sorted.
+      }
+
+      (* Now use helper lemma *)
+      apply sorted_app_smaller.
+      * exact H_rev_sorted.
+      * (* Show h <= all elements in rev (h' :: t') *)
+        intros y H_in.
+
+        (* Use our lemma to convert In y (rev (h' :: t')) to In y (h' :: t') *)
+        assert (H_in_orig: In y (h' :: t')).
+        { rewrite <- in_rev_iff. exact H_in. }
+
+        (* Now use sorted_head_le_all to show h <= y *)
+        apply sorted_head_le_all with (l := h' :: t').
+        -- exact H.
+        -- exact H_in_orig.
+Qed.
